code/Rubik/RowFoldSrchIC.v
@@ -94,6 +94,169 @@ Local Notation frnskc :=
      F frep fsym twsym dnlo dnhi fllo flhi
      cstep xstep tomemb okmv csolved croot sroot dsrch forb fpop ishm).
 
+Local Notation fsrkL :=
+  (fsrchkL e8num e4bit fpg fsgr fsbt F frep fsym twsym dnlo dnhi fllo flhi
+     cstep xstep tomemb okmv csolved ishm).
+Local Notation fsrskL :=
+  (fsrchskL e8num e4bit fpg fsgr fsbt F frep fsym twsym dnlo dnhi fllo flhi
+     cstep xstep tomemb okmv csolved ishm).
+
+(* ---- the int searches with hcoset's last level ---------------------------- *)
+
+(* fsrchki with the last move handed straight to the search at nought        *)
+Fixpoint isrchkL (cut : bool) (togo : nat) (togoi : int) (c : int) (x : pst)
+                 (msk pv : int) (m : rmap) : rmap :=
+  if togo is togo'.+1 then
+    if togo' is 0 then
+      ifold RowRun.nmvn 0
+        (fun k m' =>
+           if Uint63.eqb (Uint63.land msk (Uint63.lsl 1 k)) 0 then m'
+           else if ~~ okmv pv k then m'
+           else if cut && ~~ Uint63.eqb (Uint63.land ishm (Uint63.lsl 1 k)) 0
+           then m'
+           else fsrki cut 0 0 (cstep c k) (xstep x k) 0 k m')
+        m
+    else
+    let togoi' := Uint63.sub togoi 1 in
+    ifold RowRun.nmvn 0
+      (fun k m' =>
+         if Uint63.eqb (Uint63.land msk (Uint63.lsl 1 k)) 0 then m'
+         else if ~~ okmv pv k then m'
+         else if (if cut
+                  then (if (togo' == 0)%N
+                        then ~~ Uint63.eqb (Uint63.land ishm
+                                              (Uint63.lsl 1 k)) 0
+                        else false)
+                  else false)
+         then m'
+         else
+           let c' := cstep c k in
+           let w := p1g c' in
+           let nd := wdist w in
+           if (if nd <=? togoi'
+               then (if cut
+                     then (if nd =? togoi' then true
+                           else frcutii <=? Uint63.add togoi' nd)
+                     else true)
+               else false)
+           then isrchkL cut togo' togoi' c' (xstep x k)
+                        (wmask w (fsslack (Uint63.sub togoi' nd))) k m'
+           else m')
+      m
+  else fsrki cut 0 togoi c x msk pv m.
+
+Fixpoint isrchskL (cut : bool) (togo : nat) (togoi : int) (c : int) (x : pst)
+                  (msk pv : int) (enough : int) (mn : rmap * int)
+                  : rmap * int :=
+  if Uint63.leb enough mn.2 then mn
+  else if togo is togo'.+1 then
+    if togo' is 0 then
+      ifold RowRun.nmvn 0
+        (fun k a =>
+           if Uint63.eqb (Uint63.land msk (Uint63.lsl 1 k)) 0 then a
+           else if ~~ okmv pv k then a
+           else if cut && ~~ Uint63.eqb (Uint63.land ishm (Uint63.lsl 1 k)) 0
+           then a
+           else fsrski cut 0 0 (cstep c k) (xstep x k) 0 k enough a)
+        mn
+    else
+    let togoi' := Uint63.sub togoi 1 in
+    ifold RowRun.nmvn 0
+      (fun k a =>
+         if Uint63.eqb (Uint63.land msk (Uint63.lsl 1 k)) 0 then a
+         else if ~~ okmv pv k then a
+         else if (if cut
+                  then (if (togo' == 0)%N
+                        then ~~ Uint63.eqb (Uint63.land ishm
+                                              (Uint63.lsl 1 k)) 0
+                        else false)
+                  else false)
+         then a
+         else
+           let c' := cstep c k in
+           let w := p1g c' in
+           let nd := wdist w in
+           if (if nd <=? togoi'
+               then (if cut
+                     then (if nd =? togoi' then true
+                           else frcutii <=? Uint63.add togoi' nd)
+                     else true)
+               else false)
+           then isrchskL cut togo' togoi' c' (xstep x k)
+                         (wmask w (fsslack (Uint63.sub togoi' nd))) k enough a
+           else a)
+      mn
+  else fsrski cut 0 togoi c x msk pv enough mn.
+
+Lemma isrchkL_eq cut togo :
+  forall togoi c x msk pv m, to_nat togoi = togo -> (togo <= 63)%N ->
+  isrchkL cut togo togoi c x msk pv m = fsrkL cut togo c x msk pv m.
+Proof.
+elim: togo => [|togo ih] togoi c x msk pv m htg hb.
+  by rewrite /isrchkL /fsrchkL; apply: fsrchki_eq.
+case: togo ih htg hb => [|togo] ih htg hb.
+  rewrite /isrchkL /fsrchkL; apply: fifold_eqf => k m'.
+  case: ifP => _; first by [].
+  case: ifP => _; first by [].
+  case: ifP => _; first by [].
+  by apply: fsrchki_eq.
+rewrite /isrchkL -/isrchkL /fsrchkL -/fsrchkL.
+cbv zeta; apply: fifold_eqf => k m'.
+have hbd : (to_nat togoi < nwB)%N := to_nat_bounded togoi.
+have h1t : (to_nat 1 <= to_nat togoi)%N by rewrite to_nat_1 htg.
+have htg' : to_nat (Uint63.sub togoi 1) = togo.+1.
+  by rewrite (to_nat_sub togoi 1 h1t hbd) to_nat_1 htg subn1.
+have ht62 : (togo.+1 <= 62)%N by rewrite -ltnS.
+case: ifP => _; first by [].
+case: ifP => _; first by [].
+rewrite andE3; case: ifP => _; first by [].
+set w := mdist _.
+rewrite (fcondE cut w htg' ht62).
+case: ifP => hif; last by [].
+have hbd' : (to_nat (Uint63.sub togoi 1) < nwB)%N :=
+  to_nat_bounded (Uint63.sub togoi 1).
+have hwle : (to_nat w <= to_nat (Uint63.sub togoi 1))%N.
+  by rewrite htg'; move: hif => /andP[].
+rewrite fmmaskiE (to_nat_sub (Uint63.sub togoi 1) w hwle hbd') htg'.
+by apply: ih; [exact: htg' | exact: ltnW].
+Qed.
+
+Lemma isrchskL_eq cut togo :
+  forall togoi c x msk pv enough mn, to_nat togoi = togo -> (togo <= 63)%N ->
+  isrchskL cut togo togoi c x msk pv enough mn
+  = fsrskL cut togo c x msk pv enough mn.
+Proof.
+elim: togo => [|togo ih] togoi c x msk pv enough mn htg hb.
+  rewrite /isrchskL /fsrchskL; case: ifP => _; first by [].
+  by apply: fsrchski_eq.
+rewrite /isrchskL -/isrchskL /fsrchskL -/fsrchskL.
+case: ifP => _; first by [].
+case: togo ih htg hb => [|togo] ih htg hb.
+  apply: fifold_eqf => k a.
+  case: ifP => _; first by [].
+  case: ifP => _; first by [].
+  case: ifP => _; first by [].
+  by apply: fsrchski_eq.
+cbv zeta; apply: fifold_eqf => k a.
+have hbd : (to_nat togoi < nwB)%N := to_nat_bounded togoi.
+have h1t : (to_nat 1 <= to_nat togoi)%N by rewrite to_nat_1 htg.
+have htg' : to_nat (Uint63.sub togoi 1) = togo.+1.
+  by rewrite (to_nat_sub togoi 1 h1t hbd) to_nat_1 htg subn1.
+have ht62 : (togo.+1 <= 62)%N by rewrite -ltnS.
+case: ifP => _; first by [].
+case: ifP => _; first by [].
+rewrite andE3; case: ifP => _; first by [].
+set w := mdist _.
+rewrite (fcondE cut w htg' ht62).
+case: ifP => hif; last by [].
+have hbd' : (to_nat (Uint63.sub togoi 1) < nwB)%N :=
+  to_nat_bounded (Uint63.sub togoi 1).
+have hwle : (to_nat w <= to_nat (Uint63.sub togoi 1))%N.
+  by rewrite htg'; move: hif => /andP[].
+rewrite fmmaskiE (to_nat_sub (Uint63.sub togoi 1) w hwle hbd') htg'.
+by apply: ih; [exact: htg' | exact: ltnW].
+Qed.
+
 (* flvlski's body with the map it searches given                              *)
 Definition fslvski (cut : bool) (d : nat) (m' : rmap) : rmap :=
   if (d <= dsrch)%N then
@@ -104,8 +267,8 @@ Definition fslvski (cut : bool) (d : nat) (m' : rmap) : rmap :=
       if (d == dsrch)%N then
         let n0 := fcount forb fpop m' in
         let e := Uint63.add enoughb (Uint63.div n0 enoughd) in
-        (fsrski cut d di croot sroot msk 18 e (m', n0)).1
-      else fsrki cut d di croot sroot msk 18 m'
+        (isrchskL cut d di croot sroot msk 18 e (m', n0)).1
+      else isrchkL cut d di croot sroot msk 18 m'
     else m'
   else m'.
 
@@ -131,7 +294,7 @@ rewrite fnleE hd; case: ifP => hle; last by [].
 have hbd : (to_nat (of_nat d) < nwB)%N := to_nat_bounded (of_nat d).
 have hwle : (to_nat w <= to_nat (of_nat d))%N by rewrite hd; exact: hle.
 rewrite fmmaskiE (to_nat_sub (of_nat d) w hwle hbd) hd.
-by case: ifP => _; [rewrite fsrchski_eq | rewrite fsrchki_eq].
+by case: ifP => _; [rewrite isrchskL_eq | rewrite isrchkL_eq].
 Qed.
 
 Lemma frunskic_eq n d n0 m dst : (d + n <= 63)%N ->
